Move name related definitions and lemmas to name.v

src/proof/controllers/statefulset/statefulset.v
@@ -3,6 +3,7 @@ From New.proof.string Require Export prefix_suffix.
 From New.proof.kubernetes_model Require Export get index create delete.
 From New.proof Require Export util.
 From New.proof.controllers Require Export common.
+From New.proof.controllers.statefulset Require Export name.
 From New.proof.controllers.statefulset Require Export statefulset_init.
 From New.proof.k8s_io.kubernetes.pkg Require Export controller.
 From New.proof.k8s_io.apimachinery.pkg.runtime Require Export schema.
@@ -41,232 +42,10 @@ Defined.
 Context `{!kubernetesModelG Σ}.
 Local Set Default Proof Using "All".
 
-Definition own_pod_frags γ dq (pod : PodV.t) : iProp Σ :=
-  own_meta_frag γ (PodV.key pod) pod.(PodV.ObjectMeta').(ObjectMetaV.UID') dq
-    pod.(PodV.ObjectMeta') ∗
-  own_spec_frag γ (PodV.key pod) pod.(PodV.ObjectMeta').(ObjectMetaV.UID') dq
-    (ObjectSpecV.PodSpec pod.(PodV.Spec')).
-
-Definition own_pods_frags γ dq (pods : list PodV.t) : iProp Σ :=
-  [∗ list] pod ∈ pods, own_pod_frags γ dq pod.
-
-Definition own_pvc_frags γ dq (pvc : PersistentVolumeClaimV.t) : iProp Σ :=
-  own_meta_frag γ (PersistentVolumeClaimV.key pvc)
-    pvc.(PersistentVolumeClaimV.ObjectMeta').(ObjectMetaV.UID') dq
-    pvc.(PersistentVolumeClaimV.ObjectMeta') ∗
-  own_spec_frag γ (PersistentVolumeClaimV.key pvc)
-    pvc.(PersistentVolumeClaimV.ObjectMeta').(ObjectMetaV.UID') dq
-    (ObjectSpecV.PersistentVolumeClaimSpec pvc.(PersistentVolumeClaimV.Spec')).
-
-Definition own_pvcs_frags γ dq (pvcs : list PersistentVolumeClaimV.t) : iProp Σ :=
-  [∗ list] pvc ∈ pvcs, own_pvc_frags γ dq pvc.
-
-Definition statefulset_replicas sts : nat :=
-  match sts.(StatefulSetV.Spec').(StatefulSetSpecV.Replicas') with
-  | Some replicas => sint.nat replicas
-  | None => 1%nat
-  end.
-
-Definition desired_ordinals sts : list nat :=
-  seq 0 (statefulset_replicas sts).
-
-Definition pvc_claim_template_names sts : list go_string :=
-  (λ claim_template,
-    claim_template.(PersistentVolumeClaimV.ObjectMeta').(ObjectMetaV.Name'))
-  <$> sts.(StatefulSetV.Spec').(StatefulSetSpecV.VolumeClaimTemplates').
-
-Definition desired_pvc_name sts claim_template_name ordinal : go_string :=
-  claim_template_name ++ "-"%go ++
-  sts.(StatefulSetV.ObjectMeta').(ObjectMetaV.Name') ++ "-"%go ++
-  decimal_string ordinal.
-
-Definition desired_pvc_key sts claim_template_name ordinal : KKey.t := {|
-  KKey.Kind' := PersistentVolumeClaimV.kind;
-  KKey.Namespace' := sts.(StatefulSetV.ObjectMeta').(ObjectMetaV.Namespace');
-  KKey.Name' := desired_pvc_name sts claim_template_name ordinal;
-|}.
-
-Definition desired_pvc_key_candidates sts : list KKey.t :=
-  concat (
-    (λ ordinal,
-      (λ claim_template_name, desired_pvc_key sts claim_template_name ordinal)
-      <$> pvc_claim_template_names sts)
-    <$> desired_ordinals sts
-  ).
-
-(* The official StatefulSet controller stores PVC requirements in maps keyed by
-   template name, so duplicate claim-template names collapse to one object key. *)
-Definition desired_pvc_keys sts : list KKey.t :=
-  elements (list_to_set (C:=gset KKey.t) (desired_pvc_key_candidates sts)).
-
-Lemma desired_pvc_keys_no_dup sts : NoDup (desired_pvc_keys sts).
-Proof.
-  unfold desired_pvc_keys.
-  apply NoDup_elements.
-Qed.
-
-Definition missing_pvc_keys sts (pvcs : list PersistentVolumeClaimV.t) : list KKey.t :=
-  filter (λ key, key ∉ (PersistentVolumeClaimV.key <$> pvcs)) (desired_pvc_keys sts).
-
-Definition pvcs_match sts pvcs : Prop :=
-  PersistentVolumeClaimV.key <$> pvcs ≡ₚ desired_pvc_keys sts.
-
-Definition desired_pod_name sts ordinal : go_string :=
-  sts.(StatefulSetV.ObjectMeta').(ObjectMetaV.Name') ++ "-"%go ++ decimal_string ordinal.
-
 (* TODO: complete this definition *)
 Parameter pod_match : StatefulSetV.t → PodV.t → Prop.
 Axiom pod_match_decision : ∀ sts pod, Decision (pod_match sts pod).
 #[local] Existing Instance pod_match_decision.
-
-Definition desired_pod_key sts ordinal : KKey.t := {|
-  KKey.Kind' := PodV.kind;
-  KKey.Namespace' := sts.(StatefulSetV.ObjectMeta').(ObjectMetaV.Namespace');
-  KKey.Name' := desired_pod_name sts ordinal;
-|}.
-
-Definition desired_pod_keys sts : list KKey.t :=
-  desired_pod_key sts <$> desired_ordinals sts.
-
-Definition pod_has_member_name sts pod : Prop :=
-  ∃ ordinal,
-    pod.(PodV.ObjectMeta').(ObjectMetaV.Name') = desired_pod_name sts ordinal.
-
-Definition pod_has_member_key sts pod : Prop :=
-  ∃ ordinal, PodV.key pod = desired_pod_key sts ordinal.
-
-Definition member_name_prefix sts : go_string :=
-  sts.(StatefulSetV.ObjectMeta').(ObjectMetaV.Name') ++ "-"%go.
-
-Definition parse_member_name sts pod : option nat :=
-  match New.proof.string.prefix_suffix.strip_prefix (member_name_prefix sts)
-      (pod.(PodV.ObjectMeta').(ObjectMetaV.Name')) with
-  | Some suffix => parse_canonical_decimal_string suffix
-  | None => None
-  end.
-
-Lemma parse_member_name_sound sts pod ordinal :
-  parse_member_name sts pod = Some ordinal →
-  pod.(PodV.ObjectMeta').(ObjectMetaV.Name') = desired_pod_name sts ordinal.
-Proof.
-  unfold parse_member_name.
-  destruct (New.proof.string.prefix_suffix.strip_prefix (member_name_prefix sts)
-    (pod.(PodV.ObjectMeta').(ObjectMetaV.Name'))) as [suffix|] eqn:Hstrip; [|done].
-  intros Hparse.
-  apply parse_canonical_decimal_string_sound in Hparse.
-  apply New.proof.string.prefix_suffix.strip_prefix_correct in Hstrip.
-  unfold desired_pod_name, member_name_prefix in *.
-  rewrite Hstrip.
-  rewrite -Hparse.
-  by rewrite List.app_assoc.
-Qed.
-
-Lemma parse_member_name_complete sts pod ordinal :
-  pod.(PodV.ObjectMeta').(ObjectMetaV.Name') = desired_pod_name sts ordinal →
-  parse_member_name sts pod = Some ordinal.
-Proof.
-  intros Hname.
-  unfold parse_member_name.
-  rewrite Hname.
-  unfold desired_pod_name, member_name_prefix.
-  rewrite List.app_assoc.
-  rewrite New.proof.string.prefix_suffix.strip_prefix_complete.
-  apply parse_canonical_decimal_string_decimal_string.
-Qed.
-
-#[local] Instance pod_has_member_name_decision sts pod :
-  Decision (pod_has_member_name sts pod).
-Proof.
-  destruct (parse_member_name sts pod) as [ordinal|] eqn:Hparse.
-  - left. exists ordinal. by apply parse_member_name_sound.
-  - right. intros [ordinal Hname].
-    apply parse_member_name_complete in Hname.
-    congruence.
-Defined.
-
-Lemma pod_has_member_key_iff sts pod :
-  pod_has_member_key sts pod ↔
-  pod.(PodV.ObjectMeta').(ObjectMetaV.Namespace') =
-    sts.(StatefulSetV.ObjectMeta').(ObjectMetaV.Namespace') ∧
-  pod_has_member_name sts pod.
-Proof.
-  split.
-  - intros [ordinal Hkey].
-    split.
-    + apply (f_equal KKey.Namespace') in Hkey. exact Hkey.
-    + exists ordinal.
-      apply (f_equal KKey.Name') in Hkey. exact Hkey.
-  - intros [Hnamespace [ordinal Hname]].
-    exists ordinal.
-    unfold PodV.key, PodV.meta_key, desired_pod_key.
-    simpl. by rewrite Hnamespace Hname.
-Qed.
-
-#[local] Instance pod_has_member_key_decision sts pod :
-  Decision (pod_has_member_key sts pod).
-Proof.
-  destruct (decide (
-    pod.(PodV.ObjectMeta').(ObjectMetaV.Namespace') =
-      sts.(StatefulSetV.ObjectMeta').(ObjectMetaV.Namespace') ∧
-    pod_has_member_name sts pod)) as [Hmember|Hnot_member].
-  - left. by apply pod_has_member_key_iff.
-  - right. intros Hmember_key.
-    apply Hnot_member. by apply pod_has_member_key_iff.
-Defined.
-
-Example pod_has_member_name_accepts_one sts pod :
-  pod.(PodV.ObjectMeta').(ObjectMetaV.Name') =
-    sts.(StatefulSetV.ObjectMeta').(ObjectMetaV.Name') ++ "-1"%go →
-  pod_has_member_name sts pod.
-Proof.
-  intros Hname.
-  exists 1%nat.
-  unfold desired_pod_name, decimal_string.
-  simpl.
-  exact Hname.
-Qed.
-
-Example pod_has_member_name_rejects_leading_zero sts pod :
-  pod.(PodV.ObjectMeta').(ObjectMetaV.Name') =
-    sts.(StatefulSetV.ObjectMeta').(ObjectMetaV.Name') ++ "-01"%go →
-  ¬ pod_has_member_name sts pod.
-Proof.
-  intros Hname [ordinal Hmember].
-  pose proof (parse_member_name_complete sts pod ordinal Hmember) as Hparse.
-  unfold parse_member_name, member_name_prefix in Hparse.
-  rewrite Hname in Hparse.
-  replace (sts.(StatefulSetV.ObjectMeta').(ObjectMetaV.Name') ++ "-01"%go)
-    with ((sts.(StatefulSetV.ObjectMeta').(ObjectMetaV.Name') ++ "-"%go) ++ "01"%go)
-    in Hparse by (rewrite -List.app_assoc; done).
-  rewrite New.proof.string.prefix_suffix.strip_prefix_complete in Hparse.
-  simpl in Hparse. done.
-Qed.
-
-Definition pod_key_is_desired sts key : Prop :=
-  key ∈ desired_pod_keys sts.
-
-#[local] Instance pod_key_is_desired_decision sts key :
-    Decision (pod_key_is_desired sts key).
-Proof. unfold pod_key_is_desired. apply _. Defined.
-
-Lemma desired_pod_key_inj sts : Inj (=) (=) (desired_pod_key sts).
-Proof.
-  intros ordinal1 ordinal2 Hkey.
-  apply (f_equal KKey.Name') in Hkey.
-  simpl in Hkey.
-  unfold desired_pod_name in Hkey.
-  apply app_inv_head in Hkey.
-  apply app_inv_head in Hkey.
-  by apply decimal_string_inj in Hkey.
-Qed.
-
-Lemma desired_pod_keys_no_dup sts : NoDup (desired_pod_keys sts).
-Proof.
-  unfold desired_pod_keys, desired_ordinals.
-  apply NoDup_fmap_2.
-  - apply desired_pod_key_inj.
-  - apply NoDup_seq.
-Qed.
 
 Definition missing_pod_keys sts (pods : list PodV.t) : list KKey.t :=
   filter (λ key, key ∉ (PodV.key <$> pods)) (desired_pod_keys sts).
@@ -295,11 +74,11 @@ Definition pod_distance sts pods : nat :=
   length (bad_name_pods sts pods) +
   length (alive_condemned_pods sts pods).
 
-Definition undesired_pvc_keys sts pvcs : list KKey.t :=
-  filter (λ key, key ∉ desired_pvc_keys sts) (PersistentVolumeClaimV.key <$> pvcs).
+Definition missing_pvc_keys sts (pvcs : list PersistentVolumeClaimV.t) : list KKey.t :=
+  filter (λ key, key ∉ (PersistentVolumeClaimV.key <$> pvcs)) (desired_pvc_keys sts).
 
 Definition pvc_distance sts pvcs : nat :=
-  length (missing_pvc_keys sts pvcs) + length (undesired_pvc_keys sts pvcs).
+  length (missing_pvc_keys sts pvcs).
 
 Definition match_distance sts pods pvcs : nat :=
   pod_distance sts pods + pvc_distance sts pvcs.
@@ -310,64 +89,32 @@ Definition pods_match sts pods : Prop :=
   PodV.key <$> needed_pods sts pods ≡ₚ desired_pod_keys sts ∧
   Forall (pod_match sts) (needed_pods sts pods).
 
+Definition pvcs_match sts (pvcs : list PersistentVolumeClaimV.t) : Prop :=
+  ∀ key, key ∈ desired_pvc_keys sts →
+    key ∈ (PersistentVolumeClaimV.key <$> pvcs).
+
 Definition current_state_matches sts pods pvcs : Prop :=
   pods_match sts pods ∧ pvcs_match sts pvcs.
 
-Lemma own_pods_frags_no_dup γ pods :
-  own_pods_frags γ 1 pods -∗
-  ⌜ NoDup (PodV.key <$> pods) ⌝.
-Proof.
-  iIntros "Hpods".
-  iAssert ([∗ list] pod ∈ pods,
-      own_meta_frag γ (PodV.key pod)
-        pod.(PodV.ObjectMeta').(ObjectMetaV.UID') 1 pod.(PodV.ObjectMeta'))%I
-    with "[Hpods]" as "Hpod_meta_frags".
-  { unfold own_pods_frags, own_pod_frags.
-    iInduction pods as [|pod pods] "IH".
-    - rewrite !big_sepL_nil. done.
-    - rewrite !big_sepL_cons.
-      iDestruct "Hpods" as "[(Hmeta & _) Hpods]".
-      iFrame "Hmeta".
-      iApply ("IH" with "Hpods"). }
-  iPoseProof (kview.own_meta_list_no_dup PodV.key PodV.ObjectMeta'
-    with "Hpod_meta_frags") as "%Hnodup".
-  done.
-Qed.
-
-Lemma own_pvcs_frags_no_dup γ pvcs :
-  own_pvcs_frags γ 1 pvcs -∗
-  ⌜ NoDup (PersistentVolumeClaimV.key <$> pvcs) ⌝.
-Proof.
-  iIntros "Hpvcs".
-  iAssert ([∗ list] pvc ∈ pvcs,
-      own_meta_frag γ (PersistentVolumeClaimV.key pvc)
-        pvc.(PersistentVolumeClaimV.ObjectMeta').(ObjectMetaV.UID') 1
-        pvc.(PersistentVolumeClaimV.ObjectMeta'))%I
-    with "[Hpvcs]" as "Hpvc_meta_frags".
-  { unfold own_pvcs_frags, own_pvc_frags.
-    iInduction pvcs as [|pvc pvcs] "IH".
-    - rewrite !big_sepL_nil. done.
-    - rewrite !big_sepL_cons.
-      iDestruct "Hpvcs" as "[(Hmeta & _) Hpvcs]".
-      iFrame "Hmeta".
-      iApply ("IH" with "Hpvcs"). }
-  iPoseProof (kview.own_meta_list_no_dup
-    PersistentVolumeClaimV.key PersistentVolumeClaimV.ObjectMeta'
-    with "Hpvc_meta_frags") as "%Hnodup".
-  done.
-Qed.
-
 Lemma match_distance_zero_matches γ sts pods pvcs :
-  own_pods_frags γ 1 pods -∗
-  own_pvcs_frags γ 1 pvcs -∗
+  ([∗ list] pod ∈ pods, own_meta_frag γ (PodV.key pod) pod.(PodV.ObjectMeta').(ObjectMetaV.UID') 1 pod.(PodV.ObjectMeta')) -∗
   ⌜ match_distance sts pods pvcs = 0%nat ↔ current_state_matches sts pods pvcs ⌝.
 Proof.
-  iIntros "Hpods Hpvcs".
-  iPoseProof (own_pods_frags_no_dup with "Hpods") as "%Hpods_nodup".
-  iPoseProof (own_pvcs_frags_no_dup with "Hpvcs") as "%Hpvcs_nodup".
+  iIntros "Hpod_meta_frags".
+  iPoseProof (kview.own_meta_list_no_dup PodV.key PodV.ObjectMeta'
+    with "Hpod_meta_frags") as "%Hpods_nodup".
   iPureIntro.
-  pose proof (desired_pod_keys_no_dup sts) as Hdesired_pods_nodup.
-  pose proof (desired_pvc_keys_no_dup sts) as Hdesired_pvcs_nodup.
+  assert (Hdesired_pods_nodup : NoDup (desired_pod_keys sts)).
+  { unfold desired_pod_keys, desired_ordinals.
+    apply NoDup_fmap_2.
+    - intros ordinal1 ordinal2 Hkey.
+      apply (f_equal KKey.Name') in Hkey.
+      simpl in Hkey.
+      unfold desired_pod_name in Hkey.
+      apply app_inv_head in Hkey.
+      apply app_inv_head in Hkey.
+      by apply decimal_string_inj in Hkey.
+    - apply NoDup_seq. }
   split.
   - intros Hdist.
     unfold match_distance, pod_distance, pvc_distance in Hdist.
@@ -377,7 +124,6 @@ Proof.
     assert (Halive_condemned_pods :
         length (alive_condemned_pods sts pods) = 0%nat) by lia.
     assert (Hmissing_pvcs : length (missing_pvc_keys sts pvcs) = 0%nat) by lia.
-    assert (Hundesired_pvcs : length (undesired_pvc_keys sts pvcs) = 0%nat) by lia.
     assert (Hpod_good_name : ∀ pod,
         pod ∈ pods → pod_has_member_key sts pod).
     { intros pod Hpod.
@@ -439,21 +185,13 @@ Proof.
                 (needed_pods sts pods) pod);
                 [|exact Hpod_needed|exact Hnot_match].
               unfold outdated_pods in Houtdated_pods. exact Houtdated_pods.
-    + apply NoDup_Permutation; [exact Hpvcs_nodup|exact Hdesired_pvcs_nodup|].
-      intros key. split.
-      * intros Hactual.
-        destruct (decide (key ∈ desired_pvc_keys sts)) as [Hdesired|Hnot_desired]; [done|].
-        exfalso.
-        eapply (filter_length_zero_not_elem
-          (λ key, key ∉ desired_pvc_keys sts) (PersistentVolumeClaimV.key <$> pvcs) key);
-          [exact Hundesired_pvcs|exact Hactual|exact Hnot_desired].
-      * intros Hdesired.
-        destruct (decide (key ∈ PersistentVolumeClaimV.key <$> pvcs)) as [Hactual|Hnot_actual]; [done|].
-        exfalso.
-        eapply (filter_length_zero_not_elem
-          (λ key, key ∉ (PersistentVolumeClaimV.key <$> pvcs)) (desired_pvc_keys sts) key);
-          [exact Hmissing_pvcs|exact Hdesired|exact Hnot_actual].
-  - intros [[Hmember [Hcondemned [Hneeded_perm Hneeded_match]]] Hpvcs_perm].
+    + intros key Hdesired.
+      destruct (decide (key ∈ PersistentVolumeClaimV.key <$> pvcs)) as [Hactual|Hnot_actual]; [done|].
+      exfalso.
+      eapply (filter_length_zero_not_elem
+        (λ key, key ∉ (PersistentVolumeClaimV.key <$> pvcs)) (desired_pvc_keys sts) key);
+        [exact Hmissing_pvcs|exact Hdesired|exact Hnot_actual].
+  - intros [[Hmember [Hcondemned [Hneeded_perm Hneeded_match]]] Hpvcs_match].
     unfold match_distance, pod_distance, pvc_distance.
     assert (Hmissing_pods_nil : missing_pod_keys sts pods = []).
     { unfold missing_pod_keys.
@@ -486,18 +224,11 @@ Proof.
     assert (Hmissing_pvcs_nil : missing_pvc_keys sts pvcs = []).
     { unfold missing_pvc_keys.
       apply filter_none. intros key Hdesired Hnot_actual.
-      apply Hnot_actual. by rewrite Hpvcs_perm. }
-    assert (Hundesired_pvcs_nil : undesired_pvc_keys sts pvcs = []).
-    { unfold undesired_pvc_keys.
-      apply filter_none. intros key Hactual Hnot_desired.
-      apply Hnot_desired. by rewrite -Hpvcs_perm. }
+      apply Hnot_actual. by apply Hpvcs_match. }
     rewrite Hmissing_pods_nil Houtdated_pods_nil Hbad_name_pods_nil
-      Halive_condemned_pods_nil Hmissing_pvcs_nil Hundesired_pvcs_nil.
+      Halive_condemned_pods_nil Hmissing_pvcs_nil.
     done.
 Qed.
-
-Definition pod_key_set (pods : list PodV.t) : gset KKey.t :=
-  list_to_set (PodV.key <$> pods).
 
 Definition pod_meta_except_resource_version_changed
     (pods pods' : list PodV.t) : Prop :=
@@ -516,7 +247,8 @@ Definition pod_spec_changed (pods pods' : list PodV.t) : Prop :=
     pod.(PodV.Spec') ≠ pod'.(PodV.Spec').
 
 Definition pods_progress_observed (pods pods' : list PodV.t) : Prop :=
-  pod_key_set pods ≠ pod_key_set pods' ∨
+  list_to_set (C:=gset KKey.t) (PodV.key <$> pods) ≠
+    list_to_set (C:=gset KKey.t) (PodV.key <$> pods') ∨
   pod_meta_except_resource_version_changed pods pods' ∨
   pod_spec_changed pods pods'.
 
@@ -525,14 +257,15 @@ Lemma wp_syncStatefulSet_progress γ l (gv: schema.GroupVersion.t) namespace nam
       "#Hisk" ∷ is_kubernetes γ l ∗
       "#Hglobal_l" ∷ (global_addr apimodel.ModelState) ↦□ l ∗
       "#Hglobal_gv" ∷ (global_addr apps_v1.SchemeGroupVersion) ↦□ gv ∗
-      "Hown_sts_meta_frag" ∷ own_meta_frag γ (StatefulSetV.key sts) sts.(StatefulSetV.ObjectMeta').(ObjectMetaV.UID')
-        dq sts.(StatefulSetV.ObjectMeta') ∗
-      "Hown_sts_spec_frag" ∷ own_spec_frag γ (StatefulSetV.key sts) sts.(StatefulSetV.ObjectMeta').(ObjectMetaV.UID')
-        dq (ObjectSpecV.StatefulSetSpec sts.(StatefulSetV.Spec')) ∗
-      "Hown_pod_frags" ∷ own_pods_frags γ 1 pods ∗
-      "Hown_pvc_frags" ∷ own_pvcs_frags γ 1 pvcs ∗
-      "Hown_children_frag" ∷ own_children_frag γ (StatefulSetV.key sts) sts.(StatefulSetV.ObjectMeta').(ObjectMetaV.UID')
-        1 (list_to_set (PodV.key <$> pods)) ∗
+      "Hown_sts_meta_frag" ∷ own_meta_frag γ (StatefulSetV.key sts) sts.(StatefulSetV.ObjectMeta').(ObjectMetaV.UID') dq sts.(StatefulSetV.ObjectMeta') ∗
+      "Hown_sts_spec_frag" ∷ own_spec_frag γ (StatefulSetV.key sts) sts.(StatefulSetV.ObjectMeta').(ObjectMetaV.UID') dq (ObjectSpecV.StatefulSetSpec sts.(StatefulSetV.Spec')) ∗
+      "Hown_pod_frags" ∷ ([∗ list] pod ∈ pods,
+        own_meta_frag γ (PodV.key pod) pod.(PodV.ObjectMeta').(ObjectMetaV.UID') 1 pod.(PodV.ObjectMeta') ∗
+        own_spec_frag γ (PodV.key pod) pod.(PodV.ObjectMeta').(ObjectMetaV.UID') 1 (ObjectSpecV.PodSpec pod.(PodV.Spec'))) ∗
+      "Hown_pvc_frags" ∷ ([∗ list] pvc ∈ pvcs,
+        own_meta_frag γ (PersistentVolumeClaimV.key pvc) pvc.(PersistentVolumeClaimV.ObjectMeta').(ObjectMetaV.UID') 1 pvc.(PersistentVolumeClaimV.ObjectMeta') ∗
+        own_spec_frag γ (PersistentVolumeClaimV.key pvc) pvc.(PersistentVolumeClaimV.ObjectMeta').(ObjectMetaV.UID') 1 (ObjectSpecV.PersistentVolumeClaimSpec pvc.(PersistentVolumeClaimV.Spec'))) ∗
+      "Hown_children_frag" ∷ own_children_frag γ (StatefulSetV.key sts) sts.(StatefulSetV.ObjectMeta').(ObjectMetaV.UID') 1 (list_to_set (PodV.key <$> pods)) ∗
       "Hown_reserved_missing_pod_keys" ∷ ([∗ list] key ∈ missing_pod_keys sts pods, own_reserved_frag γ key) ∗
       "Hown_reserved_missing_pvc_keys" ∷ ([∗ list] key ∈ missing_pvc_keys sts pvcs, own_reserved_frag γ key) ∗
       "%Hnamespace_eq" ∷ ⌜ namespace = sts.(StatefulSetV.ObjectMeta').(ObjectMetaV.Namespace') ⌝ ∗
@@ -544,14 +277,15 @@ Lemma wp_syncStatefulSet_progress γ l (gv: schema.GroupVersion.t) namespace nam
   {{{ (pods' : list PodV.t) (pvcs' : list PersistentVolumeClaimV.t) (err : interface.t), RET #err;
       ⌜ current_state_matches sts pods' pvcs' ∨
         pods_progress_observed pods pods' ∧ match_distance sts pods pvcs > match_distance sts pods' pvcs' ⌝ ∗
-      own_meta_frag γ (StatefulSetV.key sts) sts.(StatefulSetV.ObjectMeta').(ObjectMetaV.UID')
-        dq sts.(StatefulSetV.ObjectMeta') ∗
-      own_spec_frag γ (StatefulSetV.key sts) sts.(StatefulSetV.ObjectMeta').(ObjectMetaV.UID')
-        dq (ObjectSpecV.StatefulSetSpec sts.(StatefulSetV.Spec')) ∗
-      own_pods_frags γ 1 pods' ∗
-      own_pvcs_frags γ 1 pvcs' ∗
-      own_children_frag γ (StatefulSetV.key sts) sts.(StatefulSetV.ObjectMeta').(ObjectMetaV.UID')
-        1 (list_to_set (PodV.key <$> pods'))
+      own_meta_frag γ (StatefulSetV.key sts) sts.(StatefulSetV.ObjectMeta').(ObjectMetaV.UID') dq sts.(StatefulSetV.ObjectMeta') ∗
+      own_spec_frag γ (StatefulSetV.key sts) sts.(StatefulSetV.ObjectMeta').(ObjectMetaV.UID') dq (ObjectSpecV.StatefulSetSpec sts.(StatefulSetV.Spec')) ∗
+      ([∗ list] pod ∈ pods',
+        own_meta_frag γ (PodV.key pod) pod.(PodV.ObjectMeta').(ObjectMetaV.UID') 1 pod.(PodV.ObjectMeta') ∗
+        own_spec_frag γ (PodV.key pod) pod.(PodV.ObjectMeta').(ObjectMetaV.UID') 1 (ObjectSpecV.PodSpec pod.(PodV.Spec'))) ∗
+      ([∗ list] pvc ∈ pvcs',
+        own_meta_frag γ (PersistentVolumeClaimV.key pvc) pvc.(PersistentVolumeClaimV.ObjectMeta').(ObjectMetaV.UID') 1 pvc.(PersistentVolumeClaimV.ObjectMeta') ∗
+        own_spec_frag γ (PersistentVolumeClaimV.key pvc) pvc.(PersistentVolumeClaimV.ObjectMeta').(ObjectMetaV.UID') 1 (ObjectSpecV.PersistentVolumeClaimSpec pvc.(PersistentVolumeClaimV.Spec'))) ∗
+      own_children_frag γ (StatefulSetV.key sts) sts.(StatefulSetV.ObjectMeta').(ObjectMetaV.UID') 1 (list_to_set (PodV.key <$> pods'))
   }}}.
 Proof.
 Admitted.
@@ -561,14 +295,15 @@ Lemma wp_syncStatefulSet_stability γ l (gv: schema.GroupVersion.t) namespace na
       "#Hisk" ∷ is_kubernetes γ l ∗
       "#Hglobal_l" ∷ (global_addr apimodel.ModelState) ↦□ l ∗
       "#Hglobal_gv" ∷ (global_addr apps_v1.SchemeGroupVersion) ↦□ gv ∗
-      "Hown_sts_meta_frag" ∷ own_meta_frag γ (StatefulSetV.key sts) sts.(StatefulSetV.ObjectMeta').(ObjectMetaV.UID')
-        dq sts.(StatefulSetV.ObjectMeta') ∗
-      "Hown_sts_spec_frag" ∷ own_spec_frag γ (StatefulSetV.key sts) sts.(StatefulSetV.ObjectMeta').(ObjectMetaV.UID')
-        dq (ObjectSpecV.StatefulSetSpec sts.(StatefulSetV.Spec')) ∗
-      "Hown_pod_frags" ∷ own_pods_frags γ dq pods ∗
-      "Hown_pvc_frags" ∷ own_pvcs_frags γ dq pvcs ∗
-      "Hown_children_frag" ∷ own_children_frag γ (StatefulSetV.key sts) sts.(StatefulSetV.ObjectMeta').(ObjectMetaV.UID')
-        dq (list_to_set (PodV.key <$> pods)) ∗
+      "Hown_sts_meta_frag" ∷ own_meta_frag γ (StatefulSetV.key sts) sts.(StatefulSetV.ObjectMeta').(ObjectMetaV.UID') dq sts.(StatefulSetV.ObjectMeta') ∗
+      "Hown_sts_spec_frag" ∷ own_spec_frag γ (StatefulSetV.key sts) sts.(StatefulSetV.ObjectMeta').(ObjectMetaV.UID') dq (ObjectSpecV.StatefulSetSpec sts.(StatefulSetV.Spec')) ∗
+      "Hown_pod_frags" ∷ ([∗ list] pod ∈ pods,
+        own_meta_frag γ (PodV.key pod) pod.(PodV.ObjectMeta').(ObjectMetaV.UID') dq pod.(PodV.ObjectMeta') ∗
+        own_spec_frag γ (PodV.key pod) pod.(PodV.ObjectMeta').(ObjectMetaV.UID') dq (ObjectSpecV.PodSpec pod.(PodV.Spec'))) ∗
+      "Hown_pvc_frags" ∷ ([∗ list] pvc ∈ pvcs,
+        own_meta_frag γ (PersistentVolumeClaimV.key pvc) pvc.(PersistentVolumeClaimV.ObjectMeta').(ObjectMetaV.UID') dq pvc.(PersistentVolumeClaimV.ObjectMeta') ∗
+        own_spec_frag γ (PersistentVolumeClaimV.key pvc) pvc.(PersistentVolumeClaimV.ObjectMeta').(ObjectMetaV.UID') dq (ObjectSpecV.PersistentVolumeClaimSpec pvc.(PersistentVolumeClaimV.Spec'))) ∗
+      "Hown_children_frag" ∷ own_children_frag γ (StatefulSetV.key sts) sts.(StatefulSetV.ObjectMeta').(ObjectMetaV.UID') dq (list_to_set (PodV.key <$> pods)) ∗
       "Hown_reserved_missing_pod_keys" ∷ ([∗ list] key ∈ missing_pod_keys sts pods, own_reserved_frag γ key) ∗
       "Hown_reserved_missing_pvc_keys" ∷ ([∗ list] key ∈ missing_pvc_keys sts pvcs, own_reserved_frag γ key) ∗
       "%Hnamespace_eq" ∷ ⌜ namespace = sts.(StatefulSetV.ObjectMeta').(ObjectMetaV.Namespace') ⌝ ∗
@@ -578,14 +313,15 @@ Lemma wp_syncStatefulSet_stability γ l (gv: schema.GroupVersion.t) namespace na
   }}}
     @! statefulset.syncStatefulSet #namespace #name
   {{{ RET #interface.nil;
-      own_meta_frag γ (StatefulSetV.key sts) sts.(StatefulSetV.ObjectMeta').(ObjectMetaV.UID')
-        dq sts.(StatefulSetV.ObjectMeta') ∗
-      own_spec_frag γ (StatefulSetV.key sts) sts.(StatefulSetV.ObjectMeta').(ObjectMetaV.UID')
-        dq (ObjectSpecV.StatefulSetSpec sts.(StatefulSetV.Spec')) ∗
-      own_pods_frags γ dq pods ∗
-      own_pvcs_frags γ dq pvcs ∗
-      own_children_frag γ (StatefulSetV.key sts) sts.(StatefulSetV.ObjectMeta').(ObjectMetaV.UID')
-        dq (list_to_set (PodV.key <$> pods))
+      own_meta_frag γ (StatefulSetV.key sts) sts.(StatefulSetV.ObjectMeta').(ObjectMetaV.UID') dq sts.(StatefulSetV.ObjectMeta') ∗
+      own_spec_frag γ (StatefulSetV.key sts) sts.(StatefulSetV.ObjectMeta').(ObjectMetaV.UID') dq (ObjectSpecV.StatefulSetSpec sts.(StatefulSetV.Spec')) ∗
+      ([∗ list] pod ∈ pods,
+        own_meta_frag γ (PodV.key pod) pod.(PodV.ObjectMeta').(ObjectMetaV.UID') dq pod.(PodV.ObjectMeta') ∗
+        own_spec_frag γ (PodV.key pod) pod.(PodV.ObjectMeta').(ObjectMetaV.UID') dq (ObjectSpecV.PodSpec pod.(PodV.Spec'))) ∗
+      ([∗ list] pvc ∈ pvcs,
+        own_meta_frag γ (PersistentVolumeClaimV.key pvc) pvc.(PersistentVolumeClaimV.ObjectMeta').(ObjectMetaV.UID') dq pvc.(PersistentVolumeClaimV.ObjectMeta') ∗
+        own_spec_frag γ (PersistentVolumeClaimV.key pvc) pvc.(PersistentVolumeClaimV.ObjectMeta').(ObjectMetaV.UID') dq (ObjectSpecV.PersistentVolumeClaimSpec pvc.(PersistentVolumeClaimV.Spec'))) ∗
+      own_children_frag γ (StatefulSetV.key sts) sts.(StatefulSetV.ObjectMeta').(ObjectMetaV.UID') dq (list_to_set (PodV.key <$> pods))
   }}}.
 Proof.
 Admitted.
