src/proof/controllers/statefulset/name.v
@@ -1,0 +1,174 @@
+From New.proof Require Import prelude empty_ffi.
+From New.proof.string Require Export prefix_suffix.
+From New.proof Require Export pure_objects.
+
+Definition desired_pod_name (sts : StatefulSetV.t) (ordinal : nat) : go_string :=
+  sts.(StatefulSetV.ObjectMeta').(ObjectMetaV.Name') ++ "-"%go ++ decimal_string ordinal.
+
+Definition desired_pod_key (sts : StatefulSetV.t) (ordinal : nat) : KKey.t := {|
+  KKey.Kind' := PodV.kind;
+  KKey.Namespace' := sts.(StatefulSetV.ObjectMeta').(ObjectMetaV.Namespace');
+  KKey.Name' := desired_pod_name sts ordinal;
+|}.
+
+Definition statefulset_replicas (sts : StatefulSetV.t) : nat :=
+  match sts.(StatefulSetV.Spec').(StatefulSetSpecV.Replicas') with
+  | Some replicas => sint.nat replicas
+  | None => 1%nat
+  end.
+
+Definition desired_ordinals (sts : StatefulSetV.t) : list nat :=
+  seq 0 (statefulset_replicas sts).
+
+Definition pvc_claim_template_names (sts : StatefulSetV.t) : list go_string :=
+  (λ claim_template,
+    claim_template.(PersistentVolumeClaimV.ObjectMeta').(ObjectMetaV.Name'))
+  <$> sts.(StatefulSetV.Spec').(StatefulSetSpecV.VolumeClaimTemplates').
+
+Definition desired_pvc_name sts claim_template_name ordinal : go_string :=
+  claim_template_name ++ "-"%go ++
+  sts.(StatefulSetV.ObjectMeta').(ObjectMetaV.Name') ++ "-"%go ++
+  decimal_string ordinal.
+
+Definition desired_pvc_key sts claim_template_name ordinal : KKey.t := {|
+  KKey.Kind' := PersistentVolumeClaimV.kind;
+  KKey.Namespace' := sts.(StatefulSetV.ObjectMeta').(ObjectMetaV.Namespace');
+  KKey.Name' := desired_pvc_name sts claim_template_name ordinal;
+|}.
+
+Definition desired_pvc_key_candidates sts : list KKey.t :=
+  concat (
+    (λ ordinal,
+      (λ claim_template_name, desired_pvc_key sts claim_template_name ordinal)
+      <$> pvc_claim_template_names sts)
+    <$> desired_ordinals sts
+  ).
+
+(* The official StatefulSet controller stores PVC requirements in maps keyed by
+   template name, so duplicate claim-template names collapse to one object key. *)
+Definition desired_pvc_keys sts : list KKey.t :=
+  elements (list_to_set (C:=gset KKey.t) (desired_pvc_key_candidates sts)).
+
+Definition desired_pod_keys (sts : StatefulSetV.t) : list KKey.t :=
+  desired_pod_key sts <$> desired_ordinals sts.
+
+Definition pod_key_is_desired (sts : StatefulSetV.t) (key : KKey.t) : Prop :=
+  key ∈ desired_pod_keys sts.
+
+#[global] Instance pod_key_is_desired_decision sts key :
+    Decision (pod_key_is_desired sts key).
+Proof. unfold pod_key_is_desired. apply _. Defined.
+
+Definition pod_has_member_name (sts : StatefulSetV.t) (pod : PodV.t) : Prop :=
+  ∃ ordinal,
+    pod.(PodV.ObjectMeta').(ObjectMetaV.Name') = desired_pod_name sts ordinal.
+
+Definition pod_has_member_key (sts : StatefulSetV.t) (pod : PodV.t) : Prop :=
+  ∃ ordinal, PodV.key pod = desired_pod_key sts ordinal.
+
+Definition member_name_prefix (sts : StatefulSetV.t) : go_string :=
+  sts.(StatefulSetV.ObjectMeta').(ObjectMetaV.Name') ++ "-"%go.
+
+Definition parse_member_name (sts : StatefulSetV.t) (pod : PodV.t) : option nat :=
+  match New.proof.string.prefix_suffix.strip_prefix (member_name_prefix sts)
+      (pod.(PodV.ObjectMeta').(ObjectMetaV.Name')) with
+  | Some suffix => parse_canonical_decimal_string suffix
+  | None => None
+  end.
+
+Lemma parse_member_name_sound sts pod ordinal :
+  parse_member_name sts pod = Some ordinal →
+  pod.(PodV.ObjectMeta').(ObjectMetaV.Name') = desired_pod_name sts ordinal.
+Proof.
+  unfold parse_member_name.
+  destruct (New.proof.string.prefix_suffix.strip_prefix (member_name_prefix sts)
+    (pod.(PodV.ObjectMeta').(ObjectMetaV.Name'))) as [suffix|] eqn:Hstrip; [|done].
+  intros Hparse.
+  apply parse_canonical_decimal_string_sound in Hparse.
+  apply New.proof.string.prefix_suffix.strip_prefix_correct in Hstrip.
+  unfold desired_pod_name, member_name_prefix in *.
+  rewrite Hstrip.
+  rewrite -Hparse.
+  by rewrite List.app_assoc.
+Qed.
+
+Lemma parse_member_name_complete sts pod ordinal :
+  pod.(PodV.ObjectMeta').(ObjectMetaV.Name') = desired_pod_name sts ordinal →
+  parse_member_name sts pod = Some ordinal.
+Proof.
+  intros Hname.
+  unfold parse_member_name.
+  rewrite Hname.
+  unfold desired_pod_name, member_name_prefix.
+  rewrite List.app_assoc.
+  rewrite New.proof.string.prefix_suffix.strip_prefix_complete.
+  apply parse_canonical_decimal_string_decimal_string.
+Qed.
+
+#[global] Instance pod_has_member_name_decision sts pod :
+  Decision (pod_has_member_name sts pod).
+Proof.
+  destruct (parse_member_name sts pod) as [ordinal|] eqn:Hparse.
+  - left. exists ordinal. by apply parse_member_name_sound.
+  - right. intros [ordinal Hname].
+    apply parse_member_name_complete in Hname.
+    congruence.
+Defined.
+
+Lemma pod_has_member_key_iff sts pod :
+  pod_has_member_key sts pod ↔
+  pod.(PodV.ObjectMeta').(ObjectMetaV.Namespace') =
+    sts.(StatefulSetV.ObjectMeta').(ObjectMetaV.Namespace') ∧
+  pod_has_member_name sts pod.
+Proof.
+  split.
+  - intros [ordinal Hkey].
+    split.
+    + apply (f_equal KKey.Namespace') in Hkey. exact Hkey.
+    + exists ordinal.
+      apply (f_equal KKey.Name') in Hkey. exact Hkey.
+  - intros [Hnamespace [ordinal Hname]].
+    exists ordinal.
+    unfold PodV.key, PodV.meta_key, desired_pod_key.
+    simpl. by rewrite Hnamespace Hname.
+Qed.
+
+#[global] Instance pod_has_member_key_decision sts pod :
+  Decision (pod_has_member_key sts pod).
+Proof.
+  destruct (decide (
+    pod.(PodV.ObjectMeta').(ObjectMetaV.Namespace') =
+      sts.(StatefulSetV.ObjectMeta').(ObjectMetaV.Namespace') ∧
+    pod_has_member_name sts pod)) as [Hmember|Hnot_member].
+  - left. by apply pod_has_member_key_iff.
+  - right. intros Hmember_key.
+    apply Hnot_member. by apply pod_has_member_key_iff.
+Defined.
+
+Example pod_has_member_name_accepts_one sts pod :
+  pod.(PodV.ObjectMeta').(ObjectMetaV.Name') =
+    sts.(StatefulSetV.ObjectMeta').(ObjectMetaV.Name') ++ "-1"%go →
+  pod_has_member_name sts pod.
+Proof.
+  intros Hname.
+  exists 1%nat.
+  unfold desired_pod_name, decimal_string.
+  simpl.
+  exact Hname.
+Qed.
+
+Example pod_has_member_name_rejects_leading_zero sts pod :
+  pod.(PodV.ObjectMeta').(ObjectMetaV.Name') =
+    sts.(StatefulSetV.ObjectMeta').(ObjectMetaV.Name') ++ "-01"%go →
+  ¬ pod_has_member_name sts pod.
+Proof.
+  intros Hname [ordinal Hmember].
+  pose proof (parse_member_name_complete sts pod ordinal Hmember) as Hparse.
+  unfold parse_member_name, member_name_prefix in Hparse.
+  rewrite Hname in Hparse.
+  replace (sts.(StatefulSetV.ObjectMeta').(ObjectMetaV.Name') ++ "-01"%go)
+    with ((sts.(StatefulSetV.ObjectMeta').(ObjectMetaV.Name') ++ "-"%go) ++ "01"%go)
+    in Hparse by (rewrite -List.app_assoc; done).
+  rewrite New.proof.string.prefix_suffix.strip_prefix_complete in Hparse.
+  simpl in Hparse. done.
+Qed.
